theories/interop/wrapper_wp.v
@@ -7,6 +7,7 @@ From melocoton.interop Require Import wrappersem wrapperstate.
 From iris.base_logic.lib Require Export ghost_map ghost_var.
 From iris.algebra.lib Require Import excl_auth gset_bij gmap_view.
 From iris.algebra Require Import ofe.
+From melocoton Require Import big_sepM_limited.
 From iris.proofmode Require Import proofmode.
 From melocoton.c_toy_lang Require Import lang melocoton.lang_instantiation melocoton.primitive_laws.
 From melocoton.ml_toy_lang Require Import lang melocoton.lang_instantiation  melocoton.primitive_laws.
@@ -56,7 +57,10 @@ Definition GC (θ : addr_map) : iProp Σ :=
      ∗ ⌜roots_are_live θ rootsmap⌝
      ∗ ([∗ map] a ↦ v ∈ rootsmap, (∃ w, a ↦C w)).
 
-Definition block_sim_raw l1 l2 : iProp Σ := (ghost_map_elem (K:=loc) (V:=lloc) wrapperGS_γχmap l1 DfracDiscarded l2).
+(* TODO: custom notation (like l1 ~~ML l2 )? *)
+(* l1 is a location in the ML heap. l2 is a block location.
+   They are similar if identified by χ *)
+Definition block_sim_raw (l1 : loc) (l2 : lloc) : iProp Σ := (l1 ↪[ wrapperGS_γχmap ]□ l2).
 
 Definition C_state_interp (ζ : lstore) (χ : lloc_map) (θ : addr_map) (roots : gset addr) : iProp Σ :=
   ∃  (ζfreeze ζσ ζrest : lstore) (χvirt : lloc_map) (fresh : gmap lloc unit) (σMLvirt : store),
@@ -67,13 +71,13 @@ Definition C_state_interp (ζ : lstore) (χ : lloc_map) (θ : addr_map) (roots :
   ∗ own wrapperGS_γχbij (gset_bij_auth (DfracOwn 1) (map_to_set pair χvirt))
   ∗ ghost_map_auth wrapperGS_γχmap 1 χvirt
   ∗ ghost_map_auth wrapperGS_γfresh 1 fresh
-  ∗ ([∗ map] ℓ ↦ γ ∈ χvirt, ⌜γ ∈ dom ζrest⌝ -∗ ℓ ↦M/)
+  ∗ big_sepM_limited χvirt (dom ζrest) (fun ℓ _ => ℓ ↦M/)
   ∗ ([∗ map] ℓ ↦ γ ∈ χvirt, block_sim_raw ℓ γ)
-  ∗ ([∗ map] l ↦ bb ∈ ζrest, match bb with  (i,t,b) => ⌜i = Immut⌝ -∗ ghost_map_elem (K:=lloc) (V:=block) wrapperGS_γζblock l DfracDiscarded (i,t,b) end)
+  ∗ ([∗ map] l ↦ bb ∈ ζrest, ⌜mutability bb = Immut⌝ -∗ l ↪[ wrapperGS_γζblock ]□ bb)
   ∗ ghost_var wrapperGS_γat_boundary (1/4) false
   ∗⌜freeze_lstore ζ ζfreeze
   ∧ ζfreeze = ζσ ∪ ζrest
-  ∧ dom ζσ ## dom ζrest
+  ∧ ζσ ##ₘ ζrest
   ∧ is_store_blocks χvirt σMLvirt ζσ
   ∧ is_store χvirt ζfreeze σMLvirt
   ∧ lloc_map_mono χ χvirt
@@ -88,14 +92,6 @@ Definition GC_token_remnant (roots : gset addr) : iProp Σ :=
  ∗ ghost_map_auth wrapperGS_γroots_map 1 (∅:gmap loc lval)
  ∗ ([∗ set] a ∈ roots, a O↦ None).
 
-Global Instance ζpers_pers (ζrest : lstore) : Persistent (([∗ map] l ↦ bb ∈ ζrest, match (bb:block) with  (i,t,b) => 
-    ⌜i = Immut⌝ -∗ ghost_map_elem (K:=lloc) (V:=block) wrapperGS_γζblock l DfracDiscarded (i,t,b) end)).
-Proof.
-  apply big_sepM_persistent. intros k ((i&t)&b). apply _.
-Qed.
-
-
-
 Definition ML_state_interp (ζ : lstore) (χ : lloc_map) (roots : roots_map) (memC : memory) : iProp Σ := 
   ∃  (ζσ ζrest : lstore) (fresh : gmap lloc unit) (σCvirt : memory),
     ghost_var wrapperGS_γroots_set (1/2) (dom roots)
@@ -105,12 +101,13 @@ Definition ML_state_interp (ζ : lstore) (χ : lloc_map) (roots : roots_map) (me
   ∗ own wrapperGS_γχbij (gset_bij_auth (DfracOwn 1) (map_to_set pair χ))
   ∗ ghost_map_auth wrapperGS_γχmap 1 χ
   ∗ ghost_map_auth wrapperGS_γfresh (1/2) fresh
-  ∗ ([∗ map] ℓ ↦ γ ∈ χ, ⌜γ ∈ dom ζrest⌝ -∗ ℓ ↦M/)
+  ∗ big_sepM_limited χ (dom ζrest) (fun ℓ _ => ℓ ↦M/)
   ∗ ([∗ map] ℓ ↦ γ ∈ χ, block_sim_raw ℓ γ)
-  ∗ ([∗ map] l ↦ bb ∈ ζrest, match bb with  (i,t,b) => ⌜i = Immut⌝ -∗ ghost_map_elem (K:=lloc) (V:=block) wrapperGS_γζblock l DfracDiscarded (i,t,b) end)
+  ∗ ([∗ map] l ↦ bb ∈ ζrest, ⌜mutability bb = Immut⌝ -∗ l ↪[ wrapperGS_γζblock ]□ bb)
   ∗ ghost_var wrapperGS_γat_boundary (1/2) true
+  ∗ GC_token_remnant (dom roots)
   ∗⌜ζ = ζσ ∪ ζrest
-  ∧ dom ζσ ## dom ζrest
+  ∧ ζσ ##ₘ ζrest
   ∧ gmap_inj χ
   ∧ (∀ x y, χ !! x = Some y → y ∈ dom ζ)
   ∧ (∀ x y, χ !! x = Some y → y ∈ dom fresh → False)⌝.
@@ -127,6 +124,12 @@ end.
 Notation SIC_ip := "((%nCv & HσC) & (%ζfreeze & %ζσ & %ζrest & %χvirt & %fresh & %σMLvirt &
            HAroots & HAθ & HAζbl & (%nMLv & HAσMLv & HAnMLv) & HAχbij & HAχmap & HAfresh & HAχNone & #HAχpers & #HAζpers & HAbound &
           %Hfreezeρ & %Hfreezeeq & %Hfreezedj & %Hstore_blocks & %Hstore & %Hχvirt & %Hχinj & %Hfreezeχ & %Hfreshχ & %HGCOK))".
+
+Notation SIML_ip := "((%nMLv & HσML) & (%ζσ & %ζrest & %fresh & %σCvirt &
+           HAroots & HAθ & HAζbl & (%nCv & HAσCv & HAnCv) & HAχbij & HAχmap & HAfresh & HAχNone & #HAχpers & #HAζpers & HAbound & HAGCrem &
+           %Hfreezeeq & %Hfreezedj & %Hχinj & %Hfreezeχ & %Hfreshχ))".
+
+Notation GC_ip := "(HAGCθ & HAGCbound & (%roots_s & %roots_m & HArootss & HArootsm & %Hrootsdom & %Hrootslive & Hrootspto))".
 
 Global Program Instance wrapGS :
   mlanguage.weakestpre.mlangGS hlc _ Σ wrap_lang
@@ -154,127 +157,161 @@ Next Obligation.
     * iPureIntro. congruence.
 Qed.
 
-Definition adjoin_mut (m : ismut) (p : tag * list lval) : block := match p with (p1,p2) => (m,p1,p2) end.
-
-Notation "l ↦fresh{ dq } b" := (  ghost_map_elem (K:=lloc) (V:=block) wrapperGS_γζblock l dq (adjoin_mut Mut b)
-                                ∗ ghost_map_elem (K:=lloc) (V:=unit) wrapperGS_γfresh l dq (()))%I
+Notation "l ↦fresh{ dq } b" := (  ghost_map_elem (K:=lloc) (V:=block) wrapperGS_γζblock l dq b
+                                ∗ ghost_map_elem (K:=lloc) (V:=unit) wrapperGS_γfresh l dq (())
+                                ∗ ⌜mutability b = Mut⌝)%I
   (at level 20, format "l  ↦fresh{ dq } b") : bi_scope.
-Notation "l ↦mut{ dq } b" := (  ghost_map_elem (K:=lloc) (V:=block) wrapperGS_γζblock l dq (adjoin_mut Mut b)
+Notation "l ↦mut{ dq } b" := (  ghost_map_elem (K:=lloc) (V:=block) wrapperGS_γζblock l dq b
+                              ∗ ⌜mutability b = Mut⌝
                               ∗ ∃ ll, block_sim_raw ll l)%I
   (at level 20, format "l  ↦mut{ dq } b") : bi_scope.
-Notation "l ↦imm b" := (  ghost_map_elem (K:=lloc) (V:=block) wrapperGS_γζblock l DfracDiscarded (adjoin_mut Immut b))%I
+Notation "l ↦imm b" := (  ghost_map_elem (K:=lloc) (V:=block) wrapperGS_γζblock l DfracDiscarded b
+                        ∗ ⌜mutability b = Immut⌝)%I
   (at level 20, format "l  ↦imm b") : bi_scope.
 
 Fixpoint block_sim (v : MLval) (l : lval) : iProp Σ := match v with
   (ML_lang.LitV (ML_lang.LitInt x)) => ⌜l = (Lint x)⌝
 | (ML_lang.LitV (ML_lang.LitBool b)) => ⌜l = (Lint (if b then 1 else 0))⌝
 | (ML_lang.LitV ML_lang.LitUnit) => ⌜l = (Lint 0)⌝
-| (ML_lang.LitV ML_lang.LitPoison) => False
+| (ML_lang.LitV ML_lang.LitPoison) => False (* TODO: remove poison? *)
 | (ML_lang.LitV (ML_lang.LitLoc ℓ)) => ∃ γ, ⌜l = (Lloc γ)⌝ ∗ block_sim_raw ℓ γ
-| (ML_lang.PairV v1 v2) => ∃ γ lv1 lv2, ⌜l = (Lloc γ)⌝ ∗ γ ↦imm (TagDefault, [lv1;lv2]) ∗ block_sim v1 lv1 ∗ block_sim v2 lv2
-| (ML_lang.InjLV v) => ∃ γ lv, ⌜l = (Lloc γ)⌝ ∗ γ ↦imm (TagDefault, [lv]) ∗ block_sim v lv
-| (ML_lang.InjRV v) => ∃ γ lv, ⌜l = (Lloc γ)⌝ ∗ γ ↦imm (TagInjRV, [lv]) ∗ block_sim v lv 
-| (ML_lang.RecV _ _ _) => False end.
+| (ML_lang.PairV v1 v2) => ∃ γ lv1 lv2, ⌜l = (Lloc γ)⌝ ∗ γ ↦imm (Immut, TagDefault, [lv1;lv2]) ∗ block_sim v1 lv1 ∗ block_sim v2 lv2
+| (ML_lang.InjLV v) => ∃ γ lv, ⌜l = (Lloc γ)⌝ ∗ γ ↦imm (Immut, TagDefault, [lv]) ∗ block_sim v lv
+| (ML_lang.InjRV v) => ∃ γ lv, ⌜l = (Lloc γ)⌝ ∗ γ ↦imm (Immut, TagInjRV, [lv]) ∗ block_sim v lv 
+| (ML_lang.RecV _ _ _) => False end. (* Todo: callbacks *)
 
 Global Instance block_sim_pers v l : Persistent (block_sim v l).
 Proof.
   induction v as [[x|b| | |]| | | |] in l|-*; cbn; unshelve eapply (_).
 Qed.
 
-Fixpoint block_sim_arr (v:list MLval) (l : list lval) : iProp Σ := match (v,l) with
-  (nil,nil) => True
-| (v::vr, l::lr) => block_sim v l ∗ block_sim_arr vr lr
-| _ => False end.
-
-Global Instance block_sim_arr_pers vl ll : Persistent (block_sim_arr vl ll).
-Proof.
-  induction vl in ll|-*; destruct ll; cbn; apply _.
-Qed.
+Definition block_sim_arr (vs:list MLval) (ls : list lval) : iProp Σ := [∗ list] v;l ∈ vs;ls, block_sim v l.
 
 Context (σ : Wrap.state).
 Notation SI := (weakestpre.state_interp σ).
 
-
 Lemma GC_in_C {θ}: ⊢ (SI -∗ GC θ -∗ ⌜∃ ρc mem, σ = CState ρc mem⌝)%I.
 Proof.
   destruct σ. 2: iIntros "_ _"; iPureIntro; do 2 eexists; done.
-  iIntros "((%nCv & HσC) & (%ζσ & %ζrest & %fresh & %σCvirt & HH1 & HH2 & HH3 & HH4 & HH5 & HH6 & HH7 & HH8 & HH9 & HH10 & HH11 & HH12 & HH13))".
-  iIntros "(HG1 & HG2 & HG3)". iExFalso.
+  iIntros SIML_ip. iIntros GC_ip.
   iAssert (⌜true = false⌝)%I as "%Hdone".
-  1: iApply (ghost_var_agree with "HH11 HG2").
+  1: iApply (ghost_var_agree with "HAbound HAGCbound").
   congruence.
 Qed.
 
 
 Lemma block_sim_of_ghost_state  (ζfreeze ζσ ζrest : lstore) (χvirt : lloc_map) (σMLvirt : store)
    v b :
-  ( ([∗ map] ℓ ↦ γ ∈ χvirt, block_sim_raw ℓ γ)
-  ∗ ([∗ map] l ↦ bb ∈ ζrest, match bb with  (i,t,b) => ⌜i = Immut⌝ -∗ ghost_map_elem (K:=lloc) (V:=block) wrapperGS_γζblock l DfracDiscarded (i,t,b) end)
-  ∗⌜
-  ζfreeze = ζσ ∪ ζrest
-∧ is_store_blocks χvirt σMLvirt ζσ
-∧ is_store χvirt ζfreeze σMLvirt
-∧ is_val χvirt ζfreeze v b⌝
-  ) -∗ block_sim v b.
+     ([∗ map] ℓ ↦ γ ∈ χvirt, block_sim_raw ℓ γ)
+  -∗ ([∗ map] l ↦ bb ∈ ζrest, ⌜mutability bb = Immut⌝ -∗ l ↪[ wrapperGS_γζblock ]□ bb)
+  -∗⌜ζfreeze = ζσ ∪ ζrest⌝
+  -∗⌜is_store_blocks χvirt σMLvirt ζσ⌝
+  -∗⌜is_store χvirt ζfreeze σMLvirt⌝
+  -∗⌜ζσ ##ₘ ζrest⌝
+  -∗⌜is_val χvirt ζfreeze v b⌝
+  -∗ block_sim v b.
 Proof.
-  iIntros "(H3 & H4 & %H5 & %H7 & %H8 & %HH)".
-  unfold is_store_blocks in H7. unfold is_store in H8.
-  iInduction v as [[x|bo| | |]| | | |] "IH" forall (b HH); cbn; inversion HH; try done.
-  - iExists _. iSplit; first done. iApply (big_sepM_lookup with "H3"); done.
-  - iExists γ, lv1, lv2. iSplit; first done. iSplit.
-    * iApply (big_sepM_lookup _ _ _ (Immut, TagDefault, [lv1; lv2]) with "H4").
-      eapply lookup_union_Some_inv_r. 3: done. 1: subst; apply H1.
-      destruct (ζσ !! γ) eqn:Heq; try done. destruct H7 as [H71 H72].
-      apply elem_of_dom_2 in Heq as Heq2. apply H72 in Heq2.
-      destruct Heq2 as (ll' & C2 & Heq3 & Heq4).
-      specialize (H8 _ _ _ _ Heq4 Heq3 H1). inversion H8.
-    * inversion HH; subst. iSplit. 1: iApply ("IH" with "[] H3 H4"); done. iApply ("IH1" with "[] H3 H4"); done.
-  - iExists γ, lv. iSplit; first done. iSplit.
-    * iApply (big_sepM_lookup _ _ _ (Immut, TagDefault, [lv]) with "H4").
-      eapply lookup_union_Some_inv_r. 3: done. 1: subst; apply H0.
-      destruct (ζσ !! γ) eqn:Heq; try done. destruct H7 as [H71 H72].
-      apply elem_of_dom_2 in Heq as Heq2. apply H72 in Heq2.
-      destruct Heq2 as (ll' & C2 & Heq3 & Heq4).
-      specialize (H8 _ _ _ _ Heq4 Heq3 H0). inversion H8.
-    * iApply ("IH" with "[] H3 H4"); done.
-  - iExists γ, lv. iSplit; first done. iSplit.
-    * iApply (big_sepM_lookup _ _ _ (Immut, TagInjRV, [lv]) with "H4").
-      eapply lookup_union_Some_inv_r. 3: done. 1: subst; apply H0.
-      destruct (ζσ !! γ) eqn:Heq; try done. destruct H7 as [H71 H72].
-      apply elem_of_dom_2 in Heq as Heq2. apply H72 in Heq2.
-      destruct Heq2 as (ll' & C2 & Heq3 & Heq4).
-      specialize (H8 _ _ _ _ Heq4 Heq3 H0). inversion H8.
-    * iApply ("IH" with "[] H3 H4"); done.
+  iIntros "#Hχ #Hζ %Hfreeze %Hstorebl %Hstore %Hdisj %H".
+  iInduction v as [[x|bo| | |]| | | |] "IH" forall (b H); cbn; inversion H; try done.
+  1: iExists γ; iSplit; first done; iApply (big_sepM_lookup with "Hχ"); done.
+  1: iExists γ, lv1, lv2; iSplit; first done; iSplit. 1: iSplit; last done.
+  3-4: iExists γ, lv; iSplit; first done; iSplit; first (iSplit; last done).
+  1,3,5: iApply (big_sepM_lookup with "Hζ"); try done.
+  4: iSplit.
+  4,6,7: iApply "IH". 7: iApply "IH1".
+  4-7: iPureIntro; done.
+  all: subst.
+  1: rename H2 into H1.
+  all: pose proof H1 as H1'. 
+  all: rewrite lookup_union in H1.
+  all: destruct (ζσ !! γ) eqn:Heq; rewrite Heq in H1; unfold union_with in H1; cbn in H1.
+  all: destruct (ζrest !! γ) eqn:Heq2; rewrite Heq2 in H1; try congruence.
+  1,4,7: exfalso; eapply map_disjoint_spec; done.
+  2,4,6: rewrite Heq2; done.
+  all: destruct Hstorebl as [Hstorebl1 Hstorebl2].
+  all: unfold block in *.
+  all: rewrite <- Heq in H1; apply elem_of_dom_2 in Heq; apply Hstorebl2 in Heq.
+  all: destruct Heq as (ℓ & Vs & Hχ & Hσml).
+  all: unfold is_store in Hstore.
+  all: specialize (Hstore _ _ _ _ Hσml Hχ H1').
+  all: inversion Hstore.
 Qed.
 
 Lemma block_sim_arr_of_ghost_state  (ζfreeze ζσ ζrest : lstore) (χvirt : lloc_map) (σMLvirt : store)
    vs b :
-  ( ([∗ map] ℓ ↦ γ ∈ χvirt, block_sim_raw ℓ γ)
-  ∗ ([∗ map] l ↦ bb ∈ ζrest, match bb with  (i,t,b) => ⌜i = Immut⌝ -∗ ghost_map_elem (K:=lloc) (V:=block) wrapperGS_γζblock l DfracDiscarded (i,t,b) end)
-  ∗⌜
-  ζfreeze = ζσ ∪ ζrest
-∧ is_store_blocks χvirt σMLvirt ζσ
-∧ is_store χvirt ζfreeze σMLvirt
-∧ Forall2 (is_val χvirt ζfreeze) vs b⌝
-  ) -∗ block_sim_arr vs b.
+     ([∗ map] ℓ ↦ γ ∈ χvirt, block_sim_raw ℓ γ)
+  -∗ ([∗ map] l ↦ bb ∈ ζrest, ⌜mutability bb = Immut⌝ -∗ l ↪[ wrapperGS_γζblock ]□ bb)
+  -∗⌜ζfreeze = ζσ ∪ ζrest⌝
+  -∗⌜is_store_blocks χvirt σMLvirt ζσ⌝
+  -∗⌜is_store χvirt ζfreeze σMLvirt⌝
+  -∗⌜ζσ ##ₘ ζrest⌝
+  -∗⌜Forall2 (is_val χvirt ζfreeze) vs b⌝
+  -∗ block_sim_arr vs b.
 Proof.
-  iIntros "(H3 & H4 & %H5 & %H7 & %H8 & %H1)".
-  unfold is_store_blocks in H7. unfold is_store in H8.
-  iInduction vs as [|v vs] "IH" forall (b H1).
-  1: apply Forall2_nil_inv_l in H1 as ->; done.
-  destruct b as [|b bs]. 1: by apply Forall2_cons_nil_inv in H1.
-  destruct (Forall2_cons_1 _ _ _ _ _ H1) as [HH H1']. cbn.
-  iSplit.
-  + iApply (block_sim_of_ghost_state with "[H3 H4]"). iFrame. iPureIntro. split; first apply H5. split; first apply H7. split; try done.
-  + iApply ("IH" with "[] H3 H4"); done.
+  iIntros "#Hχ #Hζ %Hfreeze %Hstorebl %Hstore %Hdisj %H".
+  iApply big_sepL2_intro; first by eapply Forall2_length.
+  iIntros "!> %k %v %l %H1 %H2".
+  iApply (block_sim_of_ghost_state with "Hχ Hζ"); try done.
+  iPureIntro. eapply Forall2_lookup_lr; done.
 Qed.
 
-Lemma ml_to_mut θ l vs: ⊢ (SI ∗ GC θ ∗ l ↦∗ vs ==∗ SI ∗ GC θ ∗ ∃ b γ, γ ↦mut{DfracOwn 1} (TagDefault,b) ∗ block_sim_raw l γ ∗ block_sim_arr vs b)%I.
+Lemma block_sim_to_ghost_state  (ζfreeze ζσ ζrest : lstore) (χvirt : lloc_map) (σMLvirt : store)
+   v b :
+     ghost_map_auth wrapperGS_γχmap 1 χvirt
+  -∗ ghost_map_auth wrapperGS_γζblock 1 ζrest
+  -∗⌜ζfreeze = ζσ ∪ ζrest⌝
+  -∗⌜is_store_blocks χvirt σMLvirt ζσ⌝
+  -∗⌜is_store χvirt ζfreeze σMLvirt⌝
+  -∗⌜ζσ ##ₘ ζrest⌝
+  -∗ block_sim v b
+  -∗⌜is_val χvirt ζfreeze v b⌝.
 Proof.
-  iIntros "(Hσ & HGC & Hl)".
+  iIntros "Hχ Hζ %Hfreeze %Hstorebl %Hstore %Hdis Hsim".
+  iInduction v as [[x|bo| | |]| | | |] "IH" forall (b); cbn.
+  all: try (iPure "Hsim" as Hsim; subst; iPureIntro; try econstructor; done).
+  1: {iDestruct "Hsim" as "(%γ & -> & Hsim)". unfold block_sim_raw.
+      iPoseProof (ghost_map_lookup with "Hχ Hsim") as "%HH".
+      iPureIntro. econstructor. done. }
+  1: iDestruct "Hsim" as "(%γ & %lv1 & %lv2 & -> & Hsim & Hlv1 & Hlv2)";
+     iPoseProof ("IH" with "Hχ Hζ Hlv1") as "%Hr1";
+     iPoseProof ("IH1" with "Hχ Hζ Hlv2") as "%Hr2".
+  2-3: iDestruct "Hsim" as "(%γ & %lv & -> & Hsim & Hlv)";
+       iPoseProof ("IH" with "Hχ Hζ Hlv") as "%Hr".
+  1-3: iDestruct "Hsim" as "(Hsim & _)";
+       iPoseProof (@ghost_map_lookup with "Hζ Hsim") as "%HH";
+       iPureIntro; econstructor; eauto; subst;
+       rewrite lookup_union; rewrite HH;
+       destruct (ζσ !! γ) eqn:Heq; rewrite Heq; try done;
+       eapply @map_disjoint_spec in Hdis; done.
+Qed.
+
+Lemma block_sim_arr_to_ghost_state  (ζfreeze ζσ ζrest : lstore) (χvirt : lloc_map) (σMLvirt : store)
+   vs bb :
+     ghost_map_auth wrapperGS_γχmap 1 χvirt
+  -∗ ghost_map_auth wrapperGS_γζblock 1 ζrest
+  -∗⌜ζfreeze = ζσ ∪ ζrest⌝
+  -∗⌜is_store_blocks χvirt σMLvirt ζσ⌝
+  -∗⌜is_store χvirt ζfreeze σMLvirt⌝
+  -∗⌜ζσ ##ₘ ζrest⌝
+  -∗ block_sim_arr vs bb
+  -∗⌜Forall2 (is_val χvirt ζfreeze) vs bb⌝.
+Proof.
+  iIntros "Hχ Hζ %Hfreeze %Hstorebl %Hstore %Hdis Hsim".
+  iPoseProof (big_sepL2_forall with "Hsim") as "(%Heq & Hsim)".
+  iAssert (⌜(∀ i x y, vs !! i = Some x → bb !! i = Some y → is_val χvirt ζfreeze x y)⌝)%I as "%HF".
+  2: iPureIntro; by apply Forall2_same_length_lookup_2.
+  iIntros (i v b H1 H2).
+  iApply (block_sim_to_ghost_state with "Hχ Hζ"); try done.
+  iApply ("Hsim" $! i v b H1 H2).
+Qed.
+
+Definition SIupt (P:iProp Σ) : iProp Σ := SI -∗ ( |==> SI ∗ P).
+
+Lemma ml_to_mut θ l vs: ⊢ (GC θ ∗ l ↦∗ vs ∗ SI ==∗ SI ∗ GC θ ∗ ∃ b γ, γ ↦mut{DfracOwn 1} (Mut,TagDefault,b) ∗ block_sim_raw l γ ∗ block_sim_arr vs b)%I.
+Proof.
+  iIntros "(HGC & Hl & Hσ)".
   iDestruct (GC_in_C with "Hσ HGC") as "%H"; destruct H as (ρc & mem & ->).
   iDestruct "Hσ" as SIC_ip.
-  unfold state_interp. cbn.
   iDestruct (gen_heap_valid with "HAσMLv Hl") as %Hlσ.
   destruct (χvirt !! l) as [ll|] eqn:Hlχ.
   2: { exfalso. 
@@ -287,8 +324,7 @@ Proof.
   1: { destruct Hstore_blocks as [Hdom Hstore_blocks]. apply Hstore_blocks. exists l, vs. split; try done. }
   apply elem_of_dom in Hllζ. destruct Hllζ as [bb Hζσll].
   iMod (ghost_map_insert _ bb with "HAζbl") as "(HAζbl & Hzz)".
-  1: { edestruct @elem_of_disjoint as [eodj _]. specialize (eodj Hfreezedj).
-       apply not_elem_of_dom. refine (eodj ll _). apply elem_of_dom. done. }
+  1: { eapply map_disjoint_Some_l; done. }
   iModIntro. iFrame "HGC".
   unfold is_store in Hstore.
   assert (ζfreeze !! ll = Some bb) as Hfreezell.
@@ -297,44 +333,37 @@ Proof.
   specialize (Hstore l vs ll bb Hlσ Hlχ Hfreezell) as Hstorel.
   inversion Hstorel; subst vs0 bb.
   iAssert (block_sim_arr vs lvs) as "#Hblock".
-  1: { iApply (block_sim_arr_of_ghost_state). iSplitR; first iApply "HAχpers". iSplitR; first iApply "HAζpers".
-       iPureIntro. split; first apply Hfreezeeq. split; first eauto. split; eauto. }
+  1: { iApply (block_sim_arr_of_ghost_state). 1: iApply "HAχpers". 1: iApply "HAζpers". all:done. }
   iAssert (block_sim_raw l ll) as "#Hraw".
   1: iApply (big_sepM_lookup with "HAχpers"); done.
+  assert (ζrest !! ll = None) as HζllNone.
+  1: eapply map_disjoint_Some_l; done.
   iAssert (⌜gset_bijective (map_to_set pair χvirt)⌝)%I as "%Hbij".
   1: { iPoseProof (own_valid with "HAχbij") as "%Hvalid". apply gset_bij_auth_valid in Hvalid. done. }
   iSplitR "Hzz". 1: iSplitL "HσC".
   + iExists _. iApply "HσC".
   + unfold C_state_interp. iExists (ζfreeze), (delete ll ζσ), (<[ll:=(Mut, TagDefault, lvs)]> ζrest).
-    iExists χvirt, fresh, (<[l:=None]> σMLvirt). iFrame.
+    iExists χvirt, fresh, (<[l:=None]> σMLvirt). iFrame. iFrame "HAχpers".
     iSplitL "HAnMLv". 1: iExists _; iFrame.
     iSplitL. 
-    1: {assert (χvirt = <[ l := ll ]> (delete l χvirt)) as Hχeq.
-        + apply map_eq_iff. intros i. destruct (decide (i = l)); subst. 1: by rewrite lookup_insert.
-          rewrite lookup_insert_ne. 1: rewrite lookup_delete_ne. all: done.
-        + iPoseProof (big_sepM_delete _ _ _ _ Hlχ) as "(Hdel & _)". iPoseProof ("Hdel" with "HAχNone") as "(_ & Hdel')".
-          rewrite {5} Hχeq. iApply (big_sepM_insert_2 with "[Hl]"). 1: iIntros "_"; done.
-          iApply (big_sepM_impl with "Hdel'"). iIntros "%k %v %Hdeleq !>  Hin %Hdom".
-          iApply "Hin". iPureIntro. apply elem_of_dom. apply elem_of_dom in Hdom. destruct Hdom as [x Hx]. destruct (decide (v = ll)).
-          2: exists x; rewrite lookup_insert_ne in Hx; done.
-          subst v. apply lookup_delete_Some in Hdeleq. destruct Hdeleq as [Hdelne Hkχ].
-          enough (l = k) by congruence. eapply gset_bijective_eq_iff. 1: apply Hbij.
-          1-2: by apply elem_of_map_to_set_pair. done. 
-        }
-    iSplitL; first iApply "HAχpers". iSplitL.
+    1: { rewrite dom_insert_L.
+         iApply (big_sepM_insert_inj with "[] [] [] [Hl] HAχNone"). 4: iApply "Hl".
+         all: iPureIntro.
+         + intros k v1 v2 H1 H2. eapply gset_bijective_eq_iff. 1: done. 1-2: eapply elem_of_map_to_set_pair; done. done.
+         + by apply not_elem_of_dom_2.
+         + done. }
+    iSplitL.
     1: { iApply big_sepM_insert.
-         + apply not_elem_of_dom. apply elem_of_dom_2 in Hζσll.
-           edestruct @elem_of_disjoint as [eodj _]. specialize (eodj Hfreezedj).
-           exact (eodj _ Hζσll).
-         + iSplit. 2: iApply "HAζpers". iIntros "%Hne"; congruence. }
-    iPureIntro. split; last split; last split; last split; last split; last split; last split; last split; last split.
-    all: try done; eauto.
+         + done.
+         + iSplit. 2: iApply "HAζpers". cbn; iIntros "%Hne"; congruence. }
+    iPureIntro. split_and!.
+    all: eauto.
     - symmetry. subst. by apply union_delete_insert.
-    - apply map_disjoint_dom_1. apply map_disjoint_insert_r_2. 1: apply lookup_delete.
-      apply map_disjoint_delete_l. apply map_disjoint_dom_2. done.
+    - apply map_disjoint_insert_r_2. 1: apply lookup_delete.
+      apply map_disjoint_delete_l. done.
     - destruct Hstore_blocks as [HL HR]. split.
-      1: rewrite dom_insert_lookup_L; try done. intros ll'.
-      destruct (decide (ll' = ll)); try subst ll'; split.
+      1: rewrite dom_insert_lookup_L; try done.
+      intros ll'. destruct (decide (ll' = ll)); try subst ll'; split.
       * intros [x Hx]%elem_of_dom. rewrite lookup_delete in Hx. done.
       * intros (ℓ & Vs & HH1 & HH2).
         enough (l = ℓ) as <-. 2: eapply gset_bijective_eq_iff. 2: apply Hbij.
@@ -356,10 +385,67 @@ Proof.
     - intros ℓ Vs γ blk HH1 HH2 HH3. eapply Hstore; try done. destruct (decide (ℓ = l)).
       1: subst ℓ; rewrite lookup_insert in HH1; done.
       rewrite lookup_insert_ne in HH1; try done.
-  + iExists lvs, ll. iFrame. iFrame "Hblock". unfold block_sim_raw.
-    iSplit; first iExists l. all: iApply  "Hraw".
+  + iExists lvs, ll. cbn. iFrame. iFrame "Hblock Hraw". iSplitL; try done.
+    iExists _; iApply "Hraw".
 Qed.
 
+
+
+Lemma mut_to_ml γ vs b θ: ⊢ (SI ∗ GC θ ∗ γ ↦mut{DfracOwn 1} (Mut,TagDefault,b) ∗ block_sim_arr vs b ==∗ SI ∗ GC θ ∗ ∃ l, l ↦∗ vs)%I.
+Proof.
+  iIntros "(Hσ & HGC & (Hl & (_ & %ℓ & #Hlℓ)) & #Hsim)".
+  iDestruct (GC_in_C with "Hσ HGC") as "%H"; destruct H as (ρc & mem & ->).
+  iDestruct "Hσ" as SIC_ip.
+  iPoseProof (block_sim_arr_to_ghost_state with "HAχmap HAζbl [] [] [] [] Hsim ") as "%Hsim".
+  1-4: iPureIntro; done.
+  iPoseProof (@ghost_map_lookup with "HAχmap Hlℓ") as "%Hχℓ".
+  iAssert (⌜gset_bijective (map_to_set pair χvirt)⌝)%I as "%Hbij".
+  1: { iPoseProof (own_valid with "HAχbij") as "%Hvalid". apply gset_bij_auth_valid in Hvalid. done. }
+  assert (gmap_inj χvirt) as Hinj.
+  1: { intros k v1 v2 Hv1 Hv2. eapply Hbij. all: apply elem_of_map_to_set_pair; done. }
+  unfold is_store_blocks in Hstore_blocks.
+  unfold is_store in Hstore.
+  iPoseProof (@ghost_map_lookup with "HAζbl Hl") as "%Hζl".
+  iPoseProof (big_sepM_delete_S with "[] [] HAχNone") as "(Hℓ & HAχNone)".
+  1: done.
+  1: iPureIntro; eapply elem_of_dom_2; done.
+  iPoseProof ("Hℓ" $! Hχℓ) as "Hℓ".
+  iDestruct (gen_heap_valid with "HAσMLv Hℓ") as "%Hlσ".
+  iMod (gen_heap_update _ _ _ (Some vs) with "HAσMLv Hℓ") as "[HAσMLv Hℓ]".
+  iMod (ghost_map_delete with "HAζbl Hl") as "HAζbl".
+  iModIntro. iFrame "HGC". iSplitR "Hℓ". 2: iExists ℓ; done.
+  cbn. iSplitL "HσC".
+  1: iExists _; iFrame.
+  unfold C_state_interp. unfold lstore.
+  iExists ζfreeze, (<[γ:=(Mut, TagDefault, b)]>ζσ), (delete γ ζrest).
+  iExists χvirt, fresh, (<[ ℓ := Some vs ]> σMLvirt).
+  iFrame. iFrame "HAχpers".
+  iSplitL "HAnMLv". 2: iSplitL. 3: iSplitL. 4: iPureIntro; split_and!; eauto.
+  + iExists _; done.
+  + rewrite dom_delete_L. iFrame.
+  + iPoseProof big_sepM_delete as "(HH & _)"; last iPoseProof ("HH" with "HAζpers") as "(_ & HAζpers2)"; done.
+  + erewrite @union_insert_delete. 3: eapply map_disjoint_Some_r. 2: apply _. all: done.
+  + apply map_disjoint_insert_l_2. 1: apply lookup_delete.
+    apply map_disjoint_delete_r. done.
+  + destruct Hstore_blocks as [Hsl Hsr]. split. 2: intros γ'; destruct (Hsr γ') as [Hsrl Hsrr]; split.
+    * rewrite <- Hsl. apply dom_insert_lookup_L. done.
+    * intros Hin. rewrite dom_insert_L in Hin. apply elem_of_union in Hin. destruct Hin as [->%elem_of_singleton|Hin2].
+      - exists ℓ, vs. split; try done. by rewrite lookup_insert.
+      - destruct (Hsrl Hin2) as (ℓ2 & Vs & H1 & H2); exists ℓ2, Vs; split; try done.
+        rewrite lookup_insert_ne; first done; congruence.
+    * intros (ℓ2 & Vs & H1 & H2). destruct (decide (ℓ2 = ℓ)) as [->|Hne].
+      - rewrite Hχℓ in H1. injection H1; intros ->. rewrite dom_insert_L. apply elem_of_union; left. by apply elem_of_singleton.
+      - rewrite dom_insert_L. apply elem_of_union; right. apply Hsrr. eexists _, _; split; try done. rewrite lookup_insert_ne in H2; done.
+  + intros ℓ1 vs1 γ1 bl1 Hs1 Hs2 Hs3. destruct (decide (ℓ = ℓ1)) as [<- | Hne].
+    * rewrite Hχℓ in Hs2. rewrite lookup_insert in Hs1. rewrite Hfreezeeq in Hs3.
+      injection Hs2; intros ->.
+      injection Hs1; intros ->.
+      apply lookup_union_Some_inv_r in Hs3.
+      2: eapply map_disjoint_Some_r; done.
+      rewrite Hζl in Hs3. injection Hs3; intros <-. econstructor. done.
+    * rewrite lookup_insert_ne in Hs1; last done. eapply Hstore; done.
+Qed.
+  
 End Embed_logic.
 
 
